Complete outline of generator proof.

examples/generators.v
@@ -1,6 +1,4 @@
 
-(* DISCLAIMER: This example will be fully outlined and cleaned up soon. *)
-
 Add LoadPath "???\syntax".
 Add LoadPath "???\type_system".
 Add LoadPath "???\substitution".
@@ -13,16 +11,17 @@ Open Scope string_scope.
 
 
 (* ========================================================================== *)
+(* This example was a whole lot more readable before type annotations. *)
 
-Definition TyA := TyInt. (* Need some wellformed type for `obvious` tactic *)
+Definition TyA := TyInt. (* When left abstract None and Some get annotations. *)
 
-Definition TyState := TyList TyA. (* Need some wellformed type for `obvious` *)
+Definition TyState := TyList TyA.
 
 Definition TyOption A := TySum TyUnit A.
 
-Definition None := Left Unit.
+Definition None := Left TyUnit TyA Unit.
 
-Definition Some a := Right a.
+Definition Some a := Right TyUnit TyA a.
 
 (* - - - - - - - - - - - - - - - - - - - - - - - - - - - - - - - - - - - - -  *)
 
@@ -50,24 +49,31 @@ Qed.
 Example eq_set_get := (EqsU (EqsØ)
   (CtxU (CtxØ) TyState)
   (TCtxU (TCtxØ) TyState)
-    (TOp "set" (Var 0) (TOp "get" Unit (TApp 0 (Var 0))))
-    (TOp "set" (Var 0) (TApp 0 (Var 1))) ).
+    (TOp "set" TyState TyUnit
+      (Var 0) (TOp "get" TyUnit TyState Unit (TApp 0 (Var 0))))
+    (TOp "set" TyState TyUnit
+      (Var 0) (TApp 0 (Var 1))) ).
 
 Example eq_weak_state := (EqsU eq_set_get
   CtxØ
   (TCtxU (TCtxØ) TyState)
-    (TOp "get" Unit (TOp "set" (Var 0) (TApp 0 (Var 1))))
-    (TOp "get" Unit (TApp 0 (Var 0))) ).
+    (TOp "get" TyUnit TyState 
+      Unit (TOp "set" TyState TyUnit (Var 0) (TApp 0 (Var 1))))
+    (TOp "get" TyUnit TyState 
+      Unit (TApp 0 (Var 0))) ).
 
 Lemma wf_eq_set_get:
   wf_eqs eq_set_get state_sig.
 Proof.
 unfold eq_set_get. unfold state_sig.
 apply WfEqsU; obvious.
-+ eapply WfTOp. simpl. reflexivity. obvious_vtype.
-  eapply WfTOp. simpl. reflexivity. obvious_vtype.
++ wft_step. simpl. reflexivity.
+  apply vsubtype_refl. obvious. apply vsubtype_refl. obvious. obvious_vtype.
+  wft_step. simpl. reflexivity.
+  apply vsubtype_refl. obvious. apply vsubtype_refl. obvious. obvious_vtype.
   eapply WfTApp. 2: simpl; reflexivity. obvious_vtype.
-+ eapply WfTOp. simpl. reflexivity. obvious_vtype.
++ wft_step. simpl. reflexivity.
+  apply vsubtype_refl. obvious. apply vsubtype_refl. obvious. obvious_vtype.
   eapply WfTApp. 2: simpl; reflexivity. obvious_vtype.
 Qed.
 
@@ -77,10 +83,13 @@ Proof.
 unfold eq_weak_state. unfold state_sig.
 apply WfEqsU; obvious.
 + apply wf_eq_set_get.
-+ eapply WfTOp. simpl. reflexivity. obvious_vtype.
-  eapply WfTOp. simpl. reflexivity. obvious_vtype.
++ wft_step. simpl. reflexivity.
+  apply vsubtype_refl. obvious. apply vsubtype_refl. obvious. obvious_vtype.
+  wft_step. simpl. reflexivity.
+  apply vsubtype_refl. obvious. apply vsubtype_refl. obvious. obvious_vtype.
   eapply WfTApp. 2: simpl; reflexivity. obvious_vtype.
-+ eapply WfTOp. simpl. reflexivity. obvious_vtype.
++ wft_step. simpl. reflexivity.
+  apply vsubtype_refl. obvious. apply vsubtype_refl. obvious. obvious_vtype.
   eapply WfTApp. 2: simpl; reflexivity. obvious_vtype.
 Qed.
 
@@ -88,12 +97,15 @@ Qed.
 
 Example eq_none_repeats := (EqsU (EqsØ)
   CtxØ (TCtxU (TCtxØ) (TyOption TyA))
-    (TOp "next" Unit 
+    (TOp "next" TyUnit (TyOption TyA) Unit 
       (TSumMatch (Var 0) 
         (TApp 0 None)
-        (TOp "next" Unit (TApp 0 (Var 0))) ))
+        (TOp "next" TyUnit (TyOption TyA) Unit
+          (TApp 0 (Var 0))) ))
     (* ~ *)
-    (TOp "next" Unit (TOp "next" Unit (TApp 0 (Var 0))) )
+    (TOp "next" TyUnit (TyOption TyA) Unit 
+      (TOp "next" TyUnit (TyOption TyA) Unit 
+        (TApp 0 (Var 0))) )
 ).
 
 Lemma wf_eq_none_repeats:
@@ -101,64 +113,64 @@ Lemma wf_eq_none_repeats:
 Proof.
 unfold eq_none_repeats. unfold next_sig.
 apply WfEqsU; obvious.
-+ wft_step. simpl. reflexivity. obvious_vtype.
++ wft_step. simpl. reflexivity. 
+  apply vsubtype_refl. obvious. apply vsubtype_refl. obvious. obvious_vtype.
   wft_step. instantiate (1:=TyA). obvious_vtype.
   wft_step. 2: simpl; reflexivity. obvious_vtype.
-  wft_step. simpl. reflexivity. obvious_vtype.
+  wft_step. simpl. reflexivity.
+  apply vsubtype_refl. obvious. apply vsubtype_refl. obvious. obvious_vtype.
   wft_step. 2: simpl; reflexivity. obvious_vtype.
-+ wft_step. simpl. reflexivity. obvious_vtype.
-  wft_step. simpl. reflexivity. obvious_vtype.
++ wft_step. simpl. reflexivity. 
+  apply vsubtype_refl. obvious. apply vsubtype_refl. obvious. obvious_vtype.
+  wft_step. simpl. reflexivity. 
+  apply vsubtype_refl. obvious. apply vsubtype_refl. obvious. obvious_vtype.
   wft_step. 2: simpl; reflexivity. obvious_vtype.
 Qed.
 
 (* - - - - - - - - - - - - - - - - - - - - - - - - - - - - - - - - - - - - -  *)
 
-Example generator_cases := CasesU (CasesØ)
+Example generator_cases A E := CasesU (CasesØ (CTy A state_sig E))
   ("next") TyUnit (TyOption TyA) (* () k -> *)
-    (Op "get" Unit 
+    (Op "get" TyUnit TyState Unit 
       (ListMatch (Var 0)
         (* [] *) (App (Var 1) None)
-        (* x::xs *) (Op "set" (Var 0)
+        (* x::xs *) (Op "set" TyState TyUnit (Var 0)
           (App (Var 4) (Some (Var 2))))
       )
     ).
 
 Lemma cases_types A E :
   wf_vtype A -> wf_eqs E state_sig ->
-  has_htype CtxØ generator_cases next_sig (CTy A state_sig E).
+  has_htype CtxØ (generator_cases A E) next_sig (CTy A state_sig E).
 Proof.
 intros wfa wfe.
 unfold generator_cases. apply TypeH; obvious.
 apply TypeCasesU.
 { apply TypeH; obvious. apply TypeCasesØ. }
-ctype_step. eapply TypeOp. simpl. reflexivity. obvious_vtype.
-ctype_step. instantiate (1:=TyA). obvious_vtype. 
+obvious_ctype. auto. ctype_step. instantiate (1:=TyA). obvious_vtype. 
 ctype_step. instantiate (1:=TyOption TyA). obvious_vtype. obvious_vtype.
-ctype_step. eapply TypeOp. simpl. reflexivity.  obvious_vtype.
-ctype_step. instantiate (1:=TyOption TyA). obvious_vtype.
+obvious_ctype. auto. ctype_step. instantiate (1:=TyOption TyA).
 all: obvious_vtype.
 Qed.
 
 (* ========================================================================== *)
 
 
-Example generator_respects A:
-  wf_vtype A ->
+Example generator_respects:
   respects
-    CtxØ generator_cases
-    next_sig (CTy A state_sig eq_weak_state) eq_none_repeats.
+    CtxØ (generator_cases TyA eq_weak_state)
+    next_sig (CTy TyA state_sig eq_weak_state) eq_none_repeats.
 Proof.
-intros wfa.
 specialize wf_eq_weak_state as wfe1.
 specialize wf_eq_none_repeats as wfe2.
 specialize wf_sig_state_sig as wfsig1.
 specialize wf_sig_next_sig as wfsig2.
 specialize WfHypØ as wfhyp.
-apply Respects; obvious. apply RespectEqsU.
-{ apply Respects; obvious. apply RespectEqsØ. }
+apply Respects; obvious. apply cases_types; obvious. apply RespectEqsU.
+apply Respects; obvious. apply cases_types; obvious. apply RespectEqsØ.
 simpl. simpl_c_subs.
 
-(* cleanup phase L *)
+(* ---------- cleanup phase L ---------- *)
 eapply ceq_trans. apply WfJudg; obvious. admit. eapply CeqOp.
 simpl. reflexivity. apply veq_refl. obvious_vtype. obvious.
 
@@ -169,41 +181,36 @@ simpl. apply veq_refl. admit. obvious.
   simpl. reflexivity. simpl. apply veq_refl. admit. auto.
   apply WfJudg; obvious. admit. apply βApp. }
 
-simpl_c_subs. eapply ceq_trans. apply WfJudg; obvious. admit. eapply CeqListMatch.
-simpl. apply veq_refl. admit. obvious. 
-{ eapply WfJudg; obvious. admit. eapply CeqSumMatch.
-  apply veq_refl. admit. obvious. apply ceq_refl. admit. obvious.
-  apply WfJudg; obvious. admit. eapply CeqOp. simpl. reflexivity.
-  apply veq_refl. admit. obvious.
-  apply WfJudg; obvious. admit. eapply CeqListMatch.
-  + apply veq_refl. admit. obvious.
-  + apply WfJudg; obvious. admit. apply βApp.
-  + instantiate (2:=TyA). apply WfJudg; obvious. admit. eapply CeqOp.
-    simpl. reflexivity. apply veq_refl. admit. obvious. 
-    apply WfJudg; obvious. admit. apply βApp. }
+simpl_c_subs. eapply ceq_trans. apply WfJudg; obvious. admit. 
+eapply CeqListMatch. simpl. apply veq_refl. admit. obvious. 
+{ eapply WfJudg; obvious. admit. eapply βMatchLeft. }
 { apply WfJudg; obvious. admit. eapply CeqOp. simpl. reflexivity.
   apply veq_refl. admit. obvious. apply WfJudg; obvious. admit.
-  eapply CeqSumMatch. instantiate (2:=TyA). apply veq_refl. admit. obvious.
-  apply ceq_refl. admit. obvious.
-  apply WfJudg; obvious. admit. eapply CeqOp. simpl. reflexivity.
-  apply veq_refl. admit. obvious. apply WfJudg; obvious. admit.
-  eapply CeqListMatch; simpl. instantiate (2:=TyA).
-  apply veq_refl. admit. obvious.
-  apply WfJudg; obvious. admit. apply βApp.
-  apply WfJudg; obvious. admit. eapply CeqOp. simpl. reflexivity.
-  apply veq_refl. admit. obvious. apply WfJudg; obvious. admit. apply βApp. }
+  eapply βMatchRight. }
 
 simpl_c_subs. apply WfJudg; obvious. admit. eapply CeqListMatch.
 instantiate (2:=TyA).
 { apply veq_refl. admit. obvious. }
-{ apply WfJudg; obvious. admit. apply βMatchLeft. }
+{ apply ceq_refl. admit. obvious. }
 { apply WfJudg; obvious. admit. eapply CeqOp. simpl. reflexivity.
-  apply veq_refl. admit. obvious. 
-  apply WfJudg; obvious. admit. apply βMatchRight. }
+  apply veq_refl. admit. obvious.
+  apply WfJudg; obvious. admit. eapply CeqOp. simpl. reflexivity.
+  apply veq_refl. admit. obvious.
+  apply WfJudg; obvious. admit. eapply CeqListMatch.
+  apply veq_refl. admit. obvious.
+  apply WfJudg; obvious. admit. eapply βApp. 
+  apply WfJudg; obvious. admit. eapply CeqOp. simpl. reflexivity.
+  apply veq_refl. admit. obvious.
+  apply WfJudg; obvious. admit. eapply βApp. }
 
-simpl_c_subs. apply ceq_sym.
+simpl_c_subs. 
+instantiate (1:=TyUnit). instantiate (1:=TyState).
+instantiate (1:=TyState). instantiate (1:=TyUnit).
+instantiate (1:=TyUnit). instantiate (1:=TyState).
+instantiate (1:=TyState). instantiate (1:=TyUnit).
+apply ceq_sym.
 
-(* cleanup phase R *)
+(* ---------- cleanup phase R ---------- *)
 eapply ceq_trans. apply WfJudg; obvious. admit. eapply CeqOp.
 simpl. reflexivity. apply veq_refl. obvious_vtype. obvious.
 
@@ -232,47 +239,54 @@ simpl. apply veq_refl. admit. obvious.
   apply veq_refl. admit. obvious. apply WfJudg; obvious. admit. apply βApp. }
 
 simpl_c_subs. apply ceq_refl. admit. obvious.
+simpl_c_subs. 
+instantiate (1:=TyUnit). instantiate (1:=TyState).
+instantiate (1:=TyState). instantiate (1:=TyUnit).
+instantiate (1:=TyUnit). instantiate (1:=TyState).
+instantiate (1:=TyUnit). instantiate (1:=TyState).
+instantiate (1:=TyState). instantiate (1:=TyUnit).
+instantiate (1:=TyState). instantiate (1:=TyUnit).
 
-(* OOTB get set weak on left side *)
+(* ---------- OOTB GetSet ---------- *)
 
 assert ( judg 
-  (CtxU CtxØ (TyFun (TyOption TyA) (CTy A state_sig eq_weak_state))) HypØ
-  (Ceq (CTy A state_sig eq_weak_state)
-    (Op "get" Unit
-      (Op "set" (Var 0)
-      (App (Fun
+  (CtxU CtxØ (TyFun (TyOption TyA) (CTy TyA state_sig eq_weak_state))) HypØ
+  (Ceq (CTy TyA state_sig eq_weak_state)
+    (Op "get" TyUnit TyState Unit
+      (Op "set" TyState TyUnit (Var 0)
+      (App (Fun TyState
         (ListMatch (Var 0)
-          (Op "get" Unit
-              (ListMatch (Var 0) (App (Var 4) (Left Unit))
-                (Op "set" (Var 0) (App (Var 7) (Right (Var 2))))))
-          (Op "set" (Var 0)
-              (Op "get" Unit
-                (ListMatch (Var 0) (App (Var 7) (Left Unit))
-                    (Op "set" (Var 0) (App (Var 10) (Right (Var 2)))))))))
+          (Op "get" TyUnit TyState Unit
+              (ListMatch (Var 0) (App (Var 4) None)
+                (Op "set" TyState TyUnit (Var 0) (App (Var 7) (Some (Var 2))))))
+          (Op "set" TyState TyUnit (Var 0)
+              (Op "get" TyUnit TyState Unit
+                (ListMatch (Var 0) (App (Var 7) None)
+                    (Op "set" TyState TyUnit (Var 0) (App (Var 10) (Some (Var 2)))))))))
         (Var 1))))
-    (Op "get" Unit
-      (App (Fun
+    (Op "get" TyUnit TyState Unit
+      (App (Fun TyState
         (ListMatch (Var 0)
-          (Op "get" Unit
-              (ListMatch (Var 0) (App (Var 3) (Left Unit))
-                (Op "set" (Var 0) (App (Var 6) (Right (Var 2))))))
-          (Op "set" (Var 0)
-              (Op "get" Unit
-                (ListMatch (Var 0) (App (Var 6) (Left Unit))
-                    (Op "set" (Var 0) (App (Var 9) (Right (Var 2)))))))))
+          (Op "get" TyUnit TyState Unit
+              (ListMatch (Var 0) (App (Var 3) None)
+                (Op "set" TyState TyUnit (Var 0) (App (Var 6) (Some (Var 2))))))
+          (Op "set" TyState TyUnit (Var 0)
+              (Op "get" TyUnit TyState Unit
+                (ListMatch (Var 0) (App (Var 6) None)
+                    (Op "set" TyState TyUnit (Var 0) (App (Var 9) (Some (Var 2)))))))))
         (Var 0))) ) ).
 { apply WfJudg; obvious. admit.
   eapply OOTB. simpl. left. eauto.
   instantiate (1:= InstU InstØ
-  (Fun
+  (Fun TyState
     (ListMatch (Var 0)
-      (Op "get" Unit
-          (ListMatch (Var 0) (App (Var 2) (Left Unit))
-            (Op "set" (Var 0) (App (Var 5) (Right (Var 2))))))
-      (Op "set" (Var 0)
-          (Op "get" Unit
-            (ListMatch (Var 0) (App (Var 5) (Left Unit))
-                (Op "set" (Var 0) (App (Var 8) (Right (Var 2)))))))))).
+      (Op "get" TyUnit TyState Unit
+          (ListMatch (Var 0) (App (Var 2) None)
+            (Op "set" TyState TyUnit (Var 0) (App (Var 5) (Some (Var 2))))))
+      (Op "set" TyState TyUnit (Var 0)
+          (Op "get" TyUnit TyState Unit
+            (ListMatch (Var 0) (App (Var 5) None)
+                (Op "set" TyState TyUnit (Var 0) (App (Var 8) (Some (Var 2)))))))))).
   admit. simpl. reflexivity. simpl. reflexivity. }
 
 (* OOTB cleanup *)
@@ -292,12 +306,15 @@ Focus 2.
 
 (* use OOTB *)
 unfold c_subs_out, c_subs in H. simpl in H. eapply ceq_trans. exact H. clear H.
+instantiate (1:=TyUnit). instantiate (1:=TyState).
+instantiate (1:=TyState). instantiate (1:=TyUnit).
 
+(* --------- continue ---------- *)
 
-(* continue *)
+eapply ceq_trans. apply WfJudg; obvious. admit. eapply CeqOp. simpl. eauto. 
+apply veq_refl. obvious_vtype. obvious.
 
-eapply ceq_trans. apply WfJudg; obvious. admit. eapply CeqOp. simpl. eauto. apply veq_refl. obvious_vtype. obvious.
-
+(* Op distributes over match statements *)
 eapply ceq_trans. eapply Op_ListMatch.
 
 all: try reflexivity. instantiate (1:=(Var 0)).
@@ -308,35 +325,37 @@ apply WfJudg; obvious. admit. eapply CeqListMatch.
 instantiate (2:=TyA). apply veq_refl. obvious_vtype. auto.
 2: apply ceq_refl; admit.
 
-(* OOTB set get *)
+(* ---------- OOTB SetGet ---------- *)
 
 assert ( judg
-  (CtxU (CtxU CtxØ (TyFun (TyOption TyA) (CTy A state_sig eq_weak_state)))
+  (CtxU (CtxU CtxØ (TyFun (TyOption TyA) (CTy TyA state_sig eq_weak_state)))
     TyState) HypØ
-  (Ceq (CTy A state_sig eq_weak_state)
-    (Op "set" (Var 0)
-        (Op "get" Unit
-          (App(Fun
-           (ListMatch (Var 0) (App (Var 4) (Left Unit))
-              (Op "set" (Var 0) (App (Var 7) (Right (Var 2)))))) (Var 0))))
-    (Op "set" (Var 0)
-      (App (Fun
-       (ListMatch (Var 0) (App (Var 3) (Left Unit))
-          (Op "set" (Var 0) (App (Var 6) (Right (Var 2)))))) (Var 1)) )
+  (Ceq (CTy TyA state_sig eq_weak_state)
+    (Op "set" TyState TyUnit (Var 0)
+        (Op "get" TyUnit TyState Unit
+          (App (Fun TyState
+           (ListMatch (Var 0) (App (Var 4) None)
+              (Op "set" TyState TyUnit (Var 0) 
+                (App (Var 7) (Some (Var 2)))))) (Var 0))))
+    (Op "set" TyState TyUnit (Var 0)
+      (App (Fun TyState
+       (ListMatch (Var 0) (App (Var 3) None)
+          (Op "set" TyState TyUnit (Var 0) 
+            (App (Var 6) (Some (Var 2)))))) (Var 1)) )
   ) ).
 { apply WfJudg; obvious. admit.
   eapply OOTB. simpl. right. left. eauto.
   instantiate (1:= InstU (InstU InstØ 
   (* First list template vars *)
-  (Fun
-    (ListMatch (Var 0) (App (Var 2) (Left Unit))
-      (Op "set" (Var 0) (App (Var 5) (Right (Var 2))))))
+  (Fun TyState
+    (ListMatch (Var 0) (App (Var 2) None)
+      (Op "set" TyState TyUnit (Var 0) (App (Var 5) (Some (Var 2))))))
   )
   (* Then regular ones from context *)
   (Var 0)).
   admit. simpl. reflexivity. simpl. reflexivity. }
 
-(* cleanup OOTB *)
+(* OOTB cleanup *)
 eapply ceq_trans in H.
 Focus 2.
   apply WfJudg; obvious. admit. eapply CeqOp. simpl. eauto.
@@ -356,14 +375,124 @@ unfold c_subs_out, c_subs in H. simpl in H. apply ceq_sym in H.
 (* use OOTB *)
 exact H.
 
-(* continue *)
+(* --------- continue ---------- *)
+
+eapply ceq_trans. apply WfJudg; obvious. admit. eapply CeqOp. simpl. eauto. 
+apply veq_refl. obvious_vtype. obvious.
+
+(* Op distributes over match statements *)
+specialize (Op_ListMatch 
+  (Var 1) (Var 0) 
+  (ListMatch (Var 1) (App (Var 2) (Left TyUnit TyA Unit))
+              (Op "set" TyState TyUnit (Var 0)
+                 (App (Var 5) (Right TyUnit TyA (Var 2)))))
+  (Op "set" TyState TyUnit (Var 0)
+    (Op "get" TyUnit TyState Unit
+      (ListMatch (Var 0) (App (Var 6) (Left TyUnit TyA Unit))
+        (Op "set" TyState TyUnit (Var 0)
+          (App (Var 9) (Right TyUnit TyA (Var 2)))))))
+  ) as pull.
+
+apply ceq_sym. eapply pull; auto; clear pull.
+instantiate (1:=TyA). obvious_vtype. obvious_vtype. admit. admit.
+instantiate (1:=TyState). instantiate (1:=TyUnit).
 
 
+(* ---------- OOTB GetSet (again) ---------- *)
 
+assert ( judg 
+  (CtxU CtxØ (TyFun (TyOption TyA) (CTy TyA state_sig eq_weak_state))) HypØ
+  (Ceq (CTy TyA state_sig eq_weak_state)
+    (Op "get" TyUnit TyState Unit
+      (Op "set" TyState TyUnit (Var 0)
+      (App (Fun TyState
+        (ListMatch (Var 0)
+          (ListMatch (Var 0) (App (Var 3) None)
+            (Op "set" TyState TyUnit (Var 0) (App (Var 6) (Some (Var 2)))))
+          (Op "set" TyState TyUnit (Var 0)
+              (Op "get" TyUnit TyState Unit
+                (ListMatch (Var 0) (App (Var 7) None)
+                    (Op "set" TyState TyUnit (Var 0) (App (Var 10) (Some (Var 2)))))))))
+        (Var 1))))
+    (Op "get" TyUnit TyState Unit
+      (App (Fun TyState
+        (ListMatch (Var 0)
+          (ListMatch (Var 0) (App (Var 2) None)
+            (Op "set" TyState TyUnit (Var 0) (App (Var 5) (Some (Var 2)))))
+          (Op "set" TyState TyUnit (Var 0)
+              (Op "get" TyUnit TyState Unit
+                (ListMatch (Var 0) (App (Var 6) None)
+                    (Op "set" TyState TyUnit (Var 0) (App (Var 9) (Some (Var 2)))))))))
+        (Var 0))) ) ).
+{ apply WfJudg; obvious. admit.
+  eapply OOTB. simpl. left. eauto.
+  instantiate (1:= InstU InstØ
+  (Fun TyState
+    (ListMatch (Var 0)
+      (ListMatch (Var 0) (App (Var 1) None)
+        (Op "set" TyState TyUnit (Var 0) (App (Var 4) (Some (Var 2)))))
+      (Op "set" TyState TyUnit (Var 0)
+          (Op "get" TyUnit TyState Unit
+            (ListMatch (Var 0) (App (Var 5) None)
+                (Op "set" TyState TyUnit (Var 0) (App (Var 8) (Some (Var 2)))))))))).
+  admit. simpl. reflexivity. simpl. reflexivity. }
 
+(* OOTB cleanup *)
+eapply ceq_trans in H.
+Focus 2.
+  apply WfJudg; obvious. admit. eapply CeqOp. simpl. eauto.
+  apply veq_refl. obvious_vtype. obvious.
+  apply WfJudg; obvious. admit. eapply CeqOp. simpl. eauto.
+  apply veq_refl. obvious_vtype. obvious. apply ceq_sym.
+  apply WfJudg; obvious. admit. apply βApp.
 
+apply ceq_sym in H. eapply ceq_trans in H.
+Focus 2.
+  apply WfJudg; obvious. admit. eapply CeqOp. simpl. eauto.
+  apply veq_refl. obvious_vtype. obvious. apply ceq_sym.
+  apply WfJudg; obvious. admit. apply βApp.
 
+unfold c_subs_out, c_subs in H. simpl in H. apply ceq_sym in H.
 
+(* use OOTB *)
+eapply ceq_trans. exact H. clear H.
+
+(* --------- continue ---------- *)
+
+eapply WfJudg; obvious. admit. eapply CeqOp. simpl. reflexivity.
+apply veq_refl. obvious_vtype. obvious.
+
+(* Do the η rule to get rid of nested lists. A bit verbose. *)
+specialize (ηList 
+  (CtxU (CtxU CtxØ (TyFun (TyOption TyA) (CTy TyA state_sig eq_weak_state)))
+     TyState) (hyp_shift HypØ 1 0)
+  (Var 0) 0
+  (ListMatch (Var 0)
+        (ListMatch (Var 0) (App (Var 2) (Left TyUnit TyA Unit))
+           (Op "set" TyState TyUnit (Var 0)
+              (App (Var 5) (Right TyUnit TyA (Var 2)))))
+        (Op "set" TyState TyUnit (Var 0)
+           (Op "get" TyUnit TyState Unit
+              (ListMatch (Var 0) (App (Var 6) (Left TyUnit TyA Unit))
+                 (Op "set" TyState TyUnit (Var 0)
+                    (App (Var 9) (Right TyUnit TyA (Var 2))))))))
+)as rule .
+unfold c_subs in rule. simpl in rule.
+
+eapply ceq_trans. eapply WfJudg; obvious. admit. apply rule. all: clear rule.
+omega. admit.
+
+(* Final cleanup *)
+eapply WfJudg; obvious. admit. eapply CeqListMatch.
+instantiate (1:=TyA). apply veq_refl. obvious_vtype. obvious.
+
+eapply ceq_trans. eapply WfJudg; obvious. admit. apply βMatchNil.
+eapply WfJudg; obvious. admit. apply βMatchNil.
+
+eapply ceq_trans. eapply WfJudg; obvious. admit. apply βMatchCons.
+simpl_c_subs. apply ceq_refl. admit. obvious.
+
+Admitted.
 
 
 
